

Memfaktorkan ekspresi aljabar

1. $6x + 9 =$

- A. $3(2x + 3)$
- B. $6(x + 1)$
- C. $3(2x + 1)$
- D. $2(3x + 9)$
- E. $9(x + 1)$

2. $8y + 12 =$

- A. $2(4y + 6)$
- B. $4(2y + 3)$
- C. $6(y + 2)$
- D. $8(y + 1)$
- E. $12(y + 1)$

3. $15a - 10b =$

- A. $5(3a - 2b)$
- B. $10(a - b)$
- C. $5(2a - b)$
- D. $15(a - b)$
- E. $5(3a - b)$

4. $21x + 14y =$

- A. $7(3x + 2y)$
- B. $14(x + y)$
- C. $7(2x + y)$
- D. $21(x + y)$
- E. $7(3x + y)$

5. $9m - 6n =$

- A. $3(3m - 2n)$
- B. $6(m - n)$
- C. $3(2m - n)$
- D. $9(m - n)$
- E. $6(3m - n)$

6. $12p + 18q =$

- A. $6(2p + 3q)$
- B. $3(4p + 6q)$
- C. $12(p + q)$
- D. $18(p + q)$
- E. $9(2p + q)$

7. $x^2 + 5x =$

- A. $x(x + 5)$
- B. $5(x + 1)$
- C. $(x + 2)(x + 3)$
- D. $(x + 1)(x + 4)$
- E. $x(x + 1)$

8. $y^2 + 7y =$

- A. $y(y + 7)$
- B. $7(y + 1)$
- C. $(y + 2)(y + 5)$
- D. $(y + 3)(y + 4)$
- E. $y(y + 1)$

9. $a^2 + 9a =$

- A. $a(a + 9)$
- B. $9(a + 1)$
- C. $(a + 3)(a + 6)$
- D. $(a + 1)(a + 8)$
- E. $a(a + 1)$

10. $b^2 + 4b =$

- A. $b(b + 4)$
- B. $4(b + 1)$
- C. $(b + 2)(b + 2)$
- D. $(b + 1)(b + 3)$
- E. $b(b + 2)$

11. $x^2 - 4x =$

- A. $x(x - 4)$
- B. $2(x - 2)$
- C. $(x - 1)(x - 3)$
- D. $(x - 2)(x - 2)$
- E. $x(x - 2)$

12. $y^2 - 6y =$

- A. $y(y - 6)$
- B. $6(y - 1)$
- C. $(y - 2)(y - 3)$
- D. $(y - 1)(y - 5)$
- E. $y(y - 2)$

13. $a^2 - 8a =$

- A. $a(a - 8)$
- B. $8(a - 1)$
- C. $(a - 2)(a - 6)$
- D. $(a - 4)(a - 4)$
- E. $a(a - 4)$

14. $m^2 + 2m =$

- A. $m(m + 2)$
- B. $2(m + 1)$
- C. $(m + 1)(m + 1)$
- D. $(m + 2)(m + 0)$
- E. $m(m + 1)$

15. $n^2 + 10n =$

- A. $n(n + 10)$
- B. $10(n + 1)$
- C. $(n + 2)(n + 8)$
- D. $(n + 5)(n + 5)$
- E. $n(n + 5)$

16. $x^2 + 6x + 9 =$

- A. $(x + 3)(x + 3)$
- B. $(x + 2)(x + 4)$

C. $(x + 1)(x + 5)$

D. $(x + 0)(x + 9)$

E. $(x + 9)(x + 1)$

17. $y^2 + 4y + 4 =$

- A. $(y + 2)(y + 2)$
- B. $(y + 1)(y + 3)$
- C. $(y + 4)(y + 0)$
- D. $(y + 1)(y + 4)$
- E. $y(y + 4)$

18. $a^2 + 6a + 9 =$

- A. $(a + 3)(a + 3)$
- B. $(a + 2)(a + 4)$
- C. $(a + 1)(a + 5)$
- D. $(a + 0)(a + 9)$
- E. $(a + 9)(a + 1)$

19. $m^2 - 6m + 9 =$

- A. $(m - 3)(m - 3)$
- B. $(m - 2)(m - 4)$
- C. $(m - 1)(m - 5)$
- D. $(m - 9)(m + 3)$
- E. $(m - 6)(m + 1)$

20. $n^2 - 4n + 4 =$

- A. $(n - 2)(n - 2)$
- B. $(n - 1)(n - 3)$
- C. $(n - 4)(n - 0)$
- D. $(n - 2)(n + 2)$
- E. $(n - 4)(n + 1)$